\subsection{2-3}
\begin{enumerate}[leftmargin=*]
    \item The \textbf{for} loop executes $n+1$ times, so the running time of
        the code is $\Theta(n)$.
    \item The naive polynomial evaluation algorithm is: \\
        \vspace{-1.5em}
        \begin{codebox}
        \Procname{$\proc{Poly-Eval}(A,x)$}
        \li $y\gets 0$
        \li \For $i\gets 1 \To \attrib{A}{length}$
            \Do
        \li     $y\gets x^{i-1}+A[i]$
            \End
        \end{codebox}
        Since it has to perform $i-1$ mutiplication and an addition at each
        iteration, the running time of $\proc{Poly-Eval}$ is:
        \begin{displaymath}
            \sum_{n=1}^{\attrib{A}{length}} i=\Theta(n^2)
        \end{displaymath}
        It is $n$ times slower than Horner's rule.
    \item \textbf{Initialization:} Piror to the first iteration, $y=0$, and
        since a summation with no terms equals to $0$, therefore the loop
        invariant holds. \\
        \textbf{Maintenance:} At the start of the iteration when $i$ reaches $t$,
        $y=\sum_{k=0}^{n-(t+1)}a_{k+t+1}x^k$. Prior to $i$ reaches $t-1$,
        \begin{align*}
            y&= a_tx^0+x\sum_{k=0}^{n-(t+1)}a_{k+t+1}x^k\\
             &= a_tx^0+\sum_{k=1}^{n-t}a_{k+t}x^k\\
             &= \sum_{k=0}^{n-t}a_{k+t}x^k
        \end{align*}
        which is the same as $\sum_{k=0}^{n-(i+1)}a_{k+i+1}x^k$, hence the
        loop invariant holds.\\
        \textbf{Termination:} $i$ reaches $-1$ when the loop terminates.
        Plug $i=-1$ into the equation, yield $y=\sum_{k=0}^{n}a_kx^k$.
    \item
\end{enumerate}
