\subsection{3.2-1}
    $f(n)$ and $g(n)$ are monotonically increasing means that if $n_1\ge n_2$,
    then $f(n_1)\ge f(n_2)$ and $g(n_1)\ge g(n_2)$. Observe that
    $f(n_1)+g(n_1)$ also greater than or equal to $f(n_2)+g(n_2)$, therefore
    $f(n)+g(n)$ is monotonically increasing. \\
    Also notice that since $g(n_1)\ge g(n_2)$, and $f(n)$ is monotonically
    increasing, so $f(g(n_1)) \ge f(g(n_2))$, consequently, $f(g(n))$ is also
    monotonically increasing. \\
    Since $f(n_1)\ge f(n_2)$, also because $f(n)$ and $g(n)$ are nonnegative,
    then $f(n_1)\cdot g(n_1)\ge f(n_2)\cdot g(n_1)$.  Moreover,
    $g(n_1)\ge g(n_2)$, therefore $f(n_1)\cdot g(n_1) \ge f(n_2)\cdot g(n_2)$,
    hence $f(n)\cdot g(n)$ is monotonically increasing.
\subsection{3.2-2}
    \begin{align*}
        a^{\log_b{c}} &= a^{\frac{\log_a{c}}{\log_a{b}}}\\
                      &= a^{\log_a{c}\log_b{a}}\\
                      &= c^{\log_b{a}}
    \end{align*}
\subsection{3.2-3}
    % To prove $\lg(n!)=\Theta(n\lg n)$, we have to
    % show that there exist positive constants $c_1$,
    % $c_2$ and $n_0$ such that $0\le c_1n\lg n\le
    % \lg(n!)\le c_2n\lg n$ for all $n\ge n_0$.\\
    % For the left part of the inequation, according
    % to Theorem 3.18 we know
    % $\lg(n!)=\lg\sqrt{2\pi n}+n\lg(n/e)+\lg(1+
    % \Theta(1/n))$, hence
    % $c_1=1/e$ satisfy the left part of the inequation
    % for all $n\ge 0$.\\
    % For the right part  of the inequation, we know
    % $c_2n\lg n=\lg n^{c_2n}$, moreover, since $\lg n$
    % is strictly increasing and $n!\le n^n$, therefore
    % $c_2=1$ can satisfy the right part of the
    % inequation for all $n\ge 0$.\\
    Since $n!=\sqrt{2\pi}n^{n+1/2}e^{-n}$,
    \begin{align*}
        \lg (n!)    &\approx    n\lg n - n + \frac{1}{2}
        \lg(2\pi n) \\
                &=(n+\frac{1}{2})\lg n -n + \frac
                {1}{2}\lg(2\pi) \\
                &\approx n\lg n -n  \\
                &=  \Theta(n\lg n)
    \end{align*}
    Since $n!/n^n=(n-1)!/n^{n-1}\ldots (n-(n-1))!/
    n^{n-(n-1)}=1/n$, so $\lim_{n\to \infty}n!/n^n=0$,
    which means $n!=o(n^n)$. \\
    We can easily verify that when $n\ge4$, $0\le c2^n \le n!$ for any
    positive constant $c$, hence $n!=\omega(2^n)$.
\subsection{3.2-4}
\subsection{3.2-5}
\subsection{3.2-6}
    Substitute the golden ratio and its conjugate in the equation, which shows
    they both satisfies the equation.
\subsection{3.2-7}
    When $i=0$,
    \begin{align*}
        F_i &= \frac{\phi^0-\hat{\phi^0}}{\sqrt{5}}\\
            &= 0
    \end{align*}
    When $i=1$,
    \begin{align*}
        F_i &= \frac{\phi^1-\hat{\phi}^1}{\sqrt{5}}\\
            &= 1
    \end{align*}
    Assume that when $i=k-1$,
    \begin{align*}
        F_i &= \frac{\phi^{k-1}-\hat{\phi}^{k-1}}{\sqrt{5}}
    \end{align*}
    and when $i=k$,
    \begin{align*}
        F_i &= \frac{\phi^{k}-\hat{\phi}^k}{\sqrt{5}}
    \end{align*}
    therefore, when $i=k+1$,
    \begin{flalign*}
        F_i &= F_k+F_{k-1} \\
            &= \frac{\phi^i-\hat{\phi}^i}{\sqrt{5}} +
                \frac{\phi^{i-1}-\hat{\phi}^{i-1}}{\sqrt{5}} \\
            &= \frac{\phi^{i-1}(\phi+1)-\hat{\phi}^{i-1}(\hat{\phi}+1)}{\sqrt{5}}\\
            &= \frac{\phi^{i-1}(\phi-\phi\hat{\phi})-\hat{\phi}^{i-1}(\hat{\phi}-\phi\hat{\phi})}{\sqrt{5}}
            &&\mbox{Since }\phi\hat{\phi}=-1\\
            &= \frac{\phi^i(1-\hat{\phi})-\hat{\phi}^i(1-\phi)}{\sqrt{5}}\\
            &= \frac{\phi^{i+1}-\hat{\phi}^{i+1}}{\sqrt{5}}
            &&\mbox{Since }\phi+\hat{\phi}=1\\
    \end{flalign*}
    In conclusion,
    \begin{align*}
        F_i &= \frac{\phi^i-\hat{\phi}^i}{\sqrt{5}}
    \end{align*}
\subsection{3.2-8}
